\documentclass[10pt, a4paper, titlepage]{article}
\usepackage[portrait, margin=0.8cm]{geometry}
\usepackage[utf8]{inputenc}
\usepackage{amsmath}
\usepackage{amssymb}
\usepackage{graphicx}
\graphicspath{{images/}}
\usepackage{float}
\usepackage{multicol}
\usepackage{sectsty}
\usepackage[none]{hyphenat}
\usepackage{caption}
\usepackage{subcaption}

%Removes equation label numbers
\makeatletter
\renewcommand\tagform@[1]{}
\makeatother

%Removes heading numbers of headers. Disable for numbers and to create table of contents.
\setcounter{secnumdepth}{0}

%Makes headers and footers empty: removes page numbers
\pagestyle{empty}

%Sets heading font sizes.
\sectionfont{\large}
\subsectionfont{\normalsize}

%Line between columns
%\setlength{\columnseprule}{0.4pt}

%\setlength{\parskip}{1em}

%Disables paragraph indents
\setlength{\parindent}{0em}

%Toggle coluumn vertical alignment
\raggedcolumns

\DeclareMathOperator\cis{cis}

\title{12 Specialist Mathematics Summarised Notes (Work in Progress)}
\author{}
\date{2022}
\begin{document}
	
\maketitle

\begin{multicols*}{3}

\section{Functions}
\subsection{Composite Functions}
Given $f:x\mapsto f(x)$ and $g:x\mapsto g(x)$, the composite function of $f$ and $g$ is:
\begin{gather}
	(f\circ g)(x)=f(g(x))\\
	\text{or}\\
	f\circ g:x\mapsto f(g(x))
\end{gather}
In general, $(f\circ g)(x)\neq (g\circ f)(x))$.

\dotfill
\subsection{Inverse Functions}
An inverse function returns the original value from the output of a function.\\
$f(x)$ has an inverse if it is one-to-one, if $f(a)=f(b)$ only when $a=b$, $\therefore$ passes the horizontal line test.\\\\
For $f^{-1}(x)$, the inverse of $f(x)$
\begin{itemize}
	\item Is a reflection of $y=f(x)$ over $y=x$.
	\item $(f\circ f^{-1})(x)=(f^{-1}\circ f)(x)=x$
	\item Domain of $f^{-1}=$ Range of $f$.
	\item Range of $f^{-1}=$ Domain of $f$.
\end{itemize}
\dotfill
\subsection{Self-Inverse Functions}
An invertible function which is symmetrical about $y=x$.
\begin{align}
	f^{-1}(x)=f(x)
\end{align}
\dotfill
\subsection{Reciprocal Functions}
A function of the form $f(x)=\frac{k}{x}$, where $k\neq 0$ is a constant.

\dotfill
\subsection{Reciprocal of Other Functions}
The reciprocal of a function $f(x)$ is $\frac{1}{f(x)}$.\\\\
\underline{Graphing $y=\frac{1}{f(x)}$ from $y=f(x)$:}
\begin{itemize}
	\item Zero $f(x)\to$ vertical asymp $\frac{1}{f(x)}$
	\item Vertical asymp $f(x)\to$ zero $\frac{1}{f(x)}$
	\item Local max $f(x)\to$ local min $\frac{1}{f(x)}$
	\item Local min $f(x)\to$ local max $\frac{1}{f(x)}$
	\item When $f(x)>0,\ \frac{1}{f(x)}>0$
	\item When $f(x)<0,\ \frac{1}{f(x)}<0$
	\item When $f(x)\to 0,\ \frac{1}{f(x)}\to \pm \infty$
	\item When $f(x)\to \pm \infty,\ \frac{1}{f(x)}\to 0$
\end{itemize}
\underline{Invariant Points:}
\\Points which do not move under a transformation occurring at $y=\pm 1$.

\dotfill
\subsection{Rational Functions}
Results from the division of one polynomial by another.\\
Vertical asymptote occurs when denominator is zero.\\
Horizontal asymptote ascertained from behaviour of graph as $|x|\to \infty$.
\begin{itemize}
	\item If the degree of denominator $>$ numerator, horizontal asymptote at $y=0$.
	\item If the degree of denominator $<$ numerator, function has slated asymptote found through polynomial division.
	\item If the degree of denominator $=$ numerator horizontal asymptote at $y=\frac{a}{b}$ where $a$ and $b$ are the leading coefficients.
\end{itemize}

\dotfill
\subsection{Absolute Value Functions}
The absolute value or modulus $|x|$ of a real number $x$ is its distance from 0 on the number line.
\begin{align}
	|x|=
	\begin{cases}
		x\quad \text{if } x\geq 0\\
		-x\quad \text{if } x\leq 0
	\end{cases}
\end{align}
Alternatively,
\begin{align}
	|x|=\sqrt{x^2}
\end{align}
\underline{Properties:}
%\begin{align}
%	&|x|\geq0&& &&|-x|=|x|&\\
%	&|x|^2=x^2&& &&|xy|=|x||y|&\\
%	&\left|\frac{x}{y}\right|=\frac{|x|}{|y|}&& &&|x-y|=|y-x|&\\
%\end{align}
\begin{itemize}
	\item $|x|\geq0$
	\item $|x|^2=x^2$
	\item $\left|\frac{x}{y}\right|=\frac{|x|}{|y|}$
	\item $|-x|=|x|$
	\item $|xy|=|x||y|$
	\item $|x-y|=|y-x|$
\end{itemize}
If $|x|=a$ where $a>0$, then $x=\pm a$.\\
If $|x|=|b|$ then $x=\pm b$.

\dotfill
\subsection{Graphs Involving the Absolute Value Function}
\underline{Graphing $y=f(|x|)$ from $y=f(x)$:}
\begin{itemize}
	\item Discard the graph for $x<0$
	\item Reflect the graph for $x\geq 0$ in the $y$-axis
	\item Points on the $y$-axis are invariant
\end{itemize}
\underline{Graphing $y=|f(x)|$ from $y=f(x)$:}
\begin{itemize}
	\item Keep the graph for $f(x)\geq 0$
	\item Reflect the graph for $f(x)<0$ in the $x$-axis
	\item Points on the $x$-axis are invariant
\end{itemize}
\hrulefill
\section{Mathematical Induction}
\subsection{The Principle of Mathematical Induction}
Suppose $P_n$ is a proposition which is defines for every integer $n\geq a$, $a\in \mathbb{Z}$. If $P_a$ is true, and if $P_{k+1}$ is true whenever $P_k$ is true, then $P_n$ is true for all $n\geq a$.

\hrulefill
\section{Complex Numbers}
\subsection{Imaginary Numbers}
A number which cannot be placed on a number line in the form $ai$ where $a\in \mathbb{R}$ and $i=\sqrt{-1}$.\\

\dotfill
\subsection{Complex Numbers}
Any number in the form $a+bi$ where $a,b\in \mathbb{R}$ and $i=\sqrt{-1}$.
\begin{gather}
	\begin{flalign}
		&\text{If}\quad z=a+bi&&
	\end{flalign}\\
	\mathfrak{Re} (z)=a\qquad \mathfrak{Im} (z)=b
\end{gather}
\dotfill
\subsection{The Complex Plane}
Complex numbers can be plotted on the complex plane or Argand plane as a vector where the $x$-axis is the real axis and the $y$-axis is the imaginary axis.
\begin{align}
	\overrightarrow{OP}=\begin{pmatrix}x\\ y\end{pmatrix}\quad \text{represents}\quad x+yi
\end{align}
\dotfill
\subsection{Complex Conjugates}
The complex conjugate of
\begin{align}
	z=a+bi\qquad \text{is}\qquad \bar{z}=a-bi
\end{align}
In the complex plane, $\bar{z}$ is the  reflection of $z$ in the real axis.

\dotfill
\subsection{Modulus and Argument}
The modulus of the complex number \\$z=a+bi$ is the length of the vector $\big(\begin{smallmatrix}a\\ b\end{smallmatrix}\big)$, which is the real number:
\begin{align}
	|z|=\sqrt{a^2+b^2}
\end{align}
The argument of $z$, $\arg{z}$ is the angle $\theta$ between the positive real axis and $\big(\begin{smallmatrix}a\\ b\end{smallmatrix}\big)$.\\
Real numbers have argument of 0 or $\pi$.\\
Purely imaginary numbers have arguement of $\frac{\pi}{2}$ or $-\frac{\pi}{2}$.\\

\underline{Properties of Modulus:}
\begin{itemize}
	\item $|\bar{z}|=|z|$
	\item $|\bar{z}|=z\bar{z}$
	\item $|z_1z_2|=|z_1||z_2|$
	\item $\left|\frac{z_1}{z_2}\right|=\frac{|z_1|}{|z_2|},\ z_2\neq 0$
	\item $|z_1z_2z_3\dots z_n|=|z_1||z_2||z_3|\dots |z_n|$
	\item $|z^n|=|z|^n,\ n\in \mathbb{Z}^+$
\end{itemize}
\dotfill
\subsection{Polar Form}
%\begin{gather}
%	\cis{\theta}=\cos{\theta}+i\sin{\theta}\\
%	\begin{flalign}
%		&\text{A complex number $z$ has polar form}&&
%	\end{flalign}\\
%	z=|z|\cis{\theta}\\
%	\begin{flalign}
%		&\text{where $\theta = \arg{z}$.}&&\\
%		&\text{The conjugate of $z$ is:}&&
%	\end{flalign}\\
%	\bar{z}=|z|\cis{-\theta}
%\end{gather}\\
\begin{align}
	\cis{\theta}=\cos{\theta}+i\sin{\theta}
\end{align}
A complex number $z$ has polar form
\begin{align}
	z=|z|\cis{\theta}
\end{align}
where $\theta = \arg{z}$.\\
The conjugate of $z$ is:
\begin{align}
	\bar{z}=|z|\cis{-\theta}
\end{align}
\underline{Properties of $\cis{\theta}$:}
\begin{itemize}
	\item $\cis{\theta}\times \cis{\phi}=\cis{(\theta +\phi )}$
	\item $\frac{\cis{\theta}}{\cis{\phi}}=\cis{(\theta -\phi )}$
	\item $\cis{(\theta -k2\pi )}=\cis{\theta},\ k\in \mathbb{Z}$
\end{itemize}
\dotfill
\subsection{Euler's Form}
\begin{align}
	e^{i\theta}=\cos{\theta}+i\sin{\theta}
\end{align}
\dotfill
\subsection{De Moivre's Theorem}
\begin{align}
	(|z|\cis{\theta})^n=|z|^n\cis{n\theta},\ \text{for all }n\in \mathbb{Q}
\end{align}
\hrulefill
\section{Trigonometric Identities}
\subsection{Angle Relationships}
%\begin{align}
%	&\sin{(-\theta)}=-\sin{\theta}&& &&\cos{(-\theta)}=\cos{\theta}&\\
%	&\sin{(\pi -\theta)}=\sin{\theta}&& &&\cos{(\pi -\theta)}=-\cos{\theta}&\\
%	&\sin{\left(\frac{\pi}{2}-\theta \right)}=\cos{\theta}&& &&\cos{\left(\frac{\pi}{2}-\theta \right)}=\sin{\theta}&
%\end{align}
\resizebox{.9\linewidth}{!}{
	\begin{minipage}{\linewidth}
		\begin{align}
			&\sin{(-\theta)}=-\sin{\theta}&& &&\cos{(-\theta)}=\cos{\theta}&\\
			&\sin{(\pi -\theta)}=\sin{\theta}&& &&\cos{(\pi -\theta)}=-\cos{\theta}&\\
			&\sin{\left(\frac{\pi}{2}-\theta \right)}=\cos{\theta}&& &&\cos{\left(\frac{\pi}{2}-\theta \right)}=\sin{\theta}&
		\end{align}
	\end{minipage}
}\\

%\begin{flalign}
%	&\quad \sin{(-\theta)}=-\sin{\theta}&&\\
%	&\quad \cos{(-\theta)}=\cos{\theta}&&\\
%	&\quad \sin{(\pi -\theta)}=\sin{\theta}&&\\
%	&\quad \cos{(\pi -\theta)}=-\cos{\theta}&&\\
%	&\quad \sin{\left(\frac{\pi}{2}-\theta \right)}=\cos{\theta}&&\\
%	&\quad \cos{\left(\frac{\pi}{2}-\theta \right)}=\sin{\theta}&&
%\end{flalign}
\dotfill
\subsection{Pythagorean Theorem}
\begin{flalign}
	&\quad \sin^2{\theta}+\cos^2{\theta}=1&&\\
	&\quad \tan^2{\theta}+1=\sec^2{\theta}&&\\
	&\quad 1+\cot^2{\theta}=\csc^2{\theta}&&
\end{flalign}
\dotfill
\subsection{Double Angle Identities}
\begin{flalign}
	\quad \sin{2\theta}&=2\sin{\theta}\cos{\theta}&&\\
	\quad \cos{2\theta}&=\cos^2{\theta}-\sin^2{\theta}&&\\
	&=1-2\sin^2{\theta}&&\\
	&=2\cos^2{\theta}-1&&\\
	\quad \tan{2\theta}&=\frac{2\tan{\theta}}{1-\tan^2{\theta}}&&
\end{flalign}
\dotfill
\subsection{Angle Sum and Difference}
\begin{flalign}
	&\quad \sin{(A\pm B)}=\sin{A}\cos{B}\pm \cos{A}\sin{B}&&\\
	&\quad \cos{(A\pm B)}=\cos{A}\cos{B}\mp \sin{A}\sin{B}&&\\
	&\quad \tan{(A\pm B)}=\frac{\tan{A}\pm \tan{B}}{1\mp \tan{A}\tan{B}}&&
\end{flalign}
\dotfill
\subsection{Sum to Product}
\resizebox{.85\linewidth}{!}{
	\begin{minipage}{\linewidth}
		\begin{flalign}
			&\quad \sin{A}\pm \sin{B}=2\sin{\left(\frac{A\pm B}{2}\right)}\cos{\left(\frac{A\mp B}{2}\right)}&&\\
			&\quad \cos{A}+\cos{B}=2\cos{\left(\frac{A+B}{2}\right)}\cos{\left(\frac{A-B}{2}\right)}&&\\
			&\quad \cos{A}-\cos{B}=-2\sin{\left(\frac{A+B}{2}\right)}\sin{\left(\frac{A-B}{2}\right)}&&
		\end{flalign}
	\end{minipage}
}\\

\dotfill
\subsection{Product to Sum}
\resizebox{.95\linewidth}{!}{
	\begin{minipage}{\linewidth}
		\begin{flalign}
			&\quad 2\sin{A}\cos{B}=\sin{(A+B)}+\sin{(A-B)}&&\\
			&\quad 2\sin{A}\sin{B}=\cos{(A-B)}-\cos{(A+B)}&&\\
			&\quad 2\cos{A}\cos{B}=\sin{(A+B)}+\cos{(A-B)}&&
		\end{flalign}
	\end{minipage}
}\\

\hrulefill
\section{Vectors}
\subsection{Vectors in Space}
Any point $P$ in space can be specified $(x,y,z)$ corresponding to steps in the $X$, $Y$ and $Z$ direction from the origin $O$.\\
The position vector of $P$ is
\begin{align}
	\overrightarrow{OP}=\begin{pmatrix}x\\ y \\z\end{pmatrix}=x\vec{i}+y\vec{k}+z\vec{k}
\end{align}
where $\vec{i}=\big(\begin{smallmatrix}1 \\0 \\0 \end{smallmatrix}\big)$, 
$\vec{j}=\big(\begin{smallmatrix}0 \\1 \\0 \end{smallmatrix}\big)$, and 
$\vec{k}=\big(\begin{smallmatrix}0 \\0 \\1 \end{smallmatrix}\big)$, the base unit vectors.

\dotfill
\subsection{The Magnitude of a Vector}
The magnitude or length of the vector $\vec{a}=\big(\begin{smallmatrix}a_1 \\a_2 \\a_3 \end{smallmatrix}\big)$ is
\begin{align}
	|\vec{a}|=\sqrt{a_1^2+a_2^2+a_3^2}
\end{align}
\dotfill
\subsection{Operations with Vectors}
\begin{gather}
	\begin{align}
		\text{If }\vec{a}=
		\begin{pmatrix}a_1\\ a_2 \\a_3\end{pmatrix}
		\text{ and }\vec{b}=
		\begin{pmatrix}b_1\\ b_2 \\b_3\end{pmatrix}
		\text{ then:}
	\end{align}\\
	\resizebox{.85\linewidth}{!}{
		\begin{minipage}{\linewidth}
			\begin{align}
				&-\vec{a}=\begin{pmatrix}-a_1\\ -a_2 \\-a_3\end{pmatrix}&& &&\vec{a}+\vec{b}=\begin{pmatrix}a_1+b_1\\ a_2+b_2 \\a_3+b_3\end{pmatrix}&\\
				&\vec{a}-\vec{b}=\begin{pmatrix}a_1-b_1\\ a_2-b_2 \\a_3-b_3\end{pmatrix}&& &&k\vec{a}=\begin{pmatrix}ka_1\\ ka_2 \\ka_3\end{pmatrix}&
			\end{align}
		\end{minipage}
	}
\end{gather}
\dotfill
\subsection{Vector Algebra}
\begin{itemize}
	\item $\vec{a}+\vec{b}=\vec{b}+\vec{a}$
	\item $(\vec{a}+\vec{b})+\vec{c}=\vec{a}+(\vec{b}+\vec{c})$
	\item $\vec{a}+\vec{0}=\vec{0}+\vec{a}$
	\item $\vec{a}+(\vec{-a})=(\vec{-a})+\vec{a}=\vec{0}$
	\item $k(\vec{a}+\vec{b})=k\vec{a}+k\vec{b}$
	\item $|k\vec{a}|=|k||\vec{a}|$
	\item If $\vec{x}+\vec{a}=\vec{b}$ then $\vec{x}=\vec{b}=\vec{a}$
	\item If $k\vec{x}=a,$ $k\neq 0$, then $\vec{x}=\frac{1}{k}\vec{a}$
\end{itemize}
\dotfill
\subsection{Vector Between Two Points}
If $A(a_1,a_2,a_3)$ and $B(b_1,b_2,b_3)$ then the position vector of $B$ relative to $A$ is 
\begin{align}
	\overrightarrow{AB}=\overrightarrow{OB}-\overrightarrow{OA}=\begin{pmatrix}b_1-a_1\\ b_2-a_2 \\b_3-a_3\end{pmatrix}
\end{align}
The distance from $A$ to $B$ Is
\resizebox{.85\linewidth}{!}{
	\begin{minipage}{\linewidth}
		\begin{align}
			|\overrightarrow{AB}|=\sqrt{(b_1-a_1)^2+(b_2-a_2)^2+(b_3-a_3)^2}
		\end{align}
	\end{minipage}
}
\subsection{Unit Vectors}
A unit vector is a vector of length 1.
\end{multicols*}
\end{document}